Analysis/Inductives.v
@@ -3,14 +3,129 @@ Require compcert.common.Memdata.
 Require Import Cosa.Interaction.Interaction.
 Require Import Cosa.Interaction.InteractionLib.
 Require Import Cosa.Abstract.Lang.
+Require Import Cosa.Abstract.Valuation.
 Require Import Cosa.Shape.Graph.
 Require Import Cosa.Shape.Summary.
 Import List.ListNotations.
+Import Coq.Classes.EquivDec.
 
 (** In this file we define the concrete instances of inductive shapes
     we are interested in. *)
 
-(** spiwack: I have few *)
+Section Schemata.
+
+  Context {name:Type} (γ_name:name -> node -> ℘ Graph.conc).
+  Hypothesis valuation_not_fixed_summary : forall α sm f,
+    central (belongs_to_summary α sm)
+            (fun ν => (ν,f) ∈ γ_name sm α).
+
+  (** In this section we define generic combinators to build inductive
+      summaries. *)
+
+  (** [fnf n] is the type of functions taking [n] argument nodes and
+      returning a rule. *)
+  Fixpoint fnf (n:nat) : Type :=
+    match n with
+    | 0 => rule name
+    | S n => Graph.node -> fnf n
+    end
+  .
+
+  (** [rule_with_new n] is the type of interaction structures
+      requiring [n] new nodes and producing a rule. *)
+  Fixpoint rule_with_new (n:nat) : fnf n -> Interaction (℘ node) (rule name) :=
+    match n with
+    | 0 => fun r => just r
+    | S n => fun r => bind with_new (fun α => rule_with_new n (r α))
+    end
+  .
+
+  (** A correction property for [rule_with_new n]: the nodes allowed
+      in the generated rule must only contain nodes in a given set and
+      the [n] new nodes. *)
+  Fixpoint rule_correct {n:nat} : fnf n -> ℘ node -> Prop :=
+    match n with
+    | 0 => fun r P => sub (Γ:=[node]) (belongs_to_graph (fst r)) P /\
+                      sub (Γ:=[node]) (belongs_to_expr (snd r)) P
+    | S n => fun r P => forall α, rule_correct (r α) (fun β => β∈P \/ β=α)
+    end
+  .
+
+  (* arnaud: déplacer dans extra? *)
+  Lemma exists_sigTr (A:Type) (F:A->Type) (P:forall x:A, F x -> Prop) :
+    (exists u:{x:A & F x}, (P (projT1 u) (projT2 u))) <->
+    (exists (x:A) (y:F x), P x y).
+  Proof.
+    split.
+    - intros [ [ x y ] h ]; simpl in *.
+      decompose_concl; eauto.
+    - intros [ x [ y h ]].
+      eexists (existT _ x y); simpl.
+      easy.
+  Qed.
+
+  (* arnaud: déplacer dans extra? *)
+  Lemma exists_sigT (A:Type) (F:A->Type) (P:{ x:A & F x} -> Prop) :
+    (exists u, P u) <->
+    (exists (x:A) (y:F x), P (existT _ x y)).
+  Proof.
+    split.
+    - intros [ [ x y ] h ]; simpl in *.
+      decompose_concl; eauto.
+    - intros [ x [ y h ]].
+      eexists (existT _ x y); simpl.
+      easy.
+  Qed.
+
+  (* arnaud: déplacer dans extra? *)
+  Lemma exists_sig (A:Type) (F:A->Prop) (P:{ x:A | F x} -> Prop) :
+    (exists u, P u) <->
+    (exists (x:A) (y:F x), P (exist _ x y)).
+  Proof.
+    split.
+    - intros [ [ x y ] h ]; simpl in *.
+      decompose_concl; eauto.
+    - intros [ x [ y h ]].
+      eexists (existT _ x y); simpl.
+      easy.
+  Qed.
+
+  Lemma γ_unfolding_with_new (u:node->unfolding name) (P:℘ node) α :
+    γ_unfolding_with γ_name P (fun α => (bind with_new (fun β => u β α))) α =
+    Join (fun β => meet (Γ:=[_]) (fun _ => β ∉ P)
+                                 (γ_unfolding_with γ_name (fun δ=>δ∈P\/δ=β) (u β) α)).
+  Proof.
+    double_sub; intros s.
+    - unfold γ_unfolding_with; simpl.
+      intros [ [ [ β hβ ] h₂ ] [ [ [] r] h₃ ]]; simpl in *.
+      decompose_concl; eauto.
+    - unfold γ_unfolding_with; simpl.
+      intros [ β [ h₁ [ c [ r h₂ ]]]].
+      rewrite ?exists_sigT,?exists_sig; simpl.
+      eexists; split.
+      { eauto. }
+      exists (fun _ => c).
+      rewrite ?exists_sigT,?exists_sig; simpl.
+      decompose_concl; eauto.
+      easy.
+  Qed.
+
+  (** The properties of [Summary.env] are verified by unfoldings of
+      the form [rule_with_new n r] *)
+
+  Lemma vnf_rule_with_new (n:nat) (r:fnf (S n)) (P:℘ node) (α:node) :
+    α ∈ P ->
+    (rule_correct (r α) P) ->
+    forall f,
+      central P
+              (fun ν => (ν,f) ∈ γ_unfolding_with γ_name P (fun α => rule_with_new n (r α)) α).
+  Proof.
+  Admitted.
+
+
+End Schemata.
+
+(** spiwack: There are few inductive at the time, until we are able to generate them. *)
 
 Inductive name :=
 | List
@@ -20,6 +135,7 @@ Inductive name :=
 Local Notation "α ≡ β" := (Lang.Abinop (Cminor.Ocmpu Integers.Ceq) α β) (at level 70).
 Local Notation "α ≠ β" := (Lang.Aunop Cminor.Onegint (α≡β)) (at level 70).
 Local Notation "0" := (Lang.Aconst (Cminor.Ointconst Int.zero)).
+Local Notation "1" := (Lang.Aconst (Cminor.Ointconst Int.one)).
 
 Definition add_chunk (offs:int) (chunk:AST.memory_chunk) : int :=
   Int.add offs (Int.repr (Memdata.size_chunk chunk))
@@ -43,8 +159,8 @@ Definition def (i:name) (α:node) : Interaction (℘ node) (Summary.rule name) :
   | ListSegment β =>
     Interaction.pi (Finite.access [
         just (Graph.NodeTree.empty _, (Avar α) ≡ (Avar β)) (** empty segment *);
-        bind with_new (fun γ => (* head *)
-        bind with_new (fun δ => (* tail *)
+        bind with_new (fun γ => (** head *)
+        bind with_new (fun δ => (** tail *)
             just (NodeTree.set α (Point_to
                     [(Int.zero,{|destination:=(γ,Int.zero);size:=AST.Mint32|});
                      (add_chunk (Int.zero) AST.Mint32,{|destination:=(δ,Int.zero);size:=AST.Mint32|})]
@@ -55,3 +171,79 @@ Definition def (i:name) (α:node) : Interaction (℘ node) (Summary.rule name) :
       ])
   end
 .
+
+(** Segments can be unfolded from the back node. *)
+Definition list_segment_backward_unfolding (β α:node) :
+   Interaction (℘ node) (Summary.rule name) :=
+  Interaction.pi (Finite.access [
+      just ( (** backward unfolding can yield identity. *)
+        NodeTree.set α (Summarized (ListSegment β))
+       (NodeTree.empty _),1 );
+
+      bind with_new (fun γ => (** value *)
+      bind with_new (fun δ => (** new end point *)
+        just (NodeTree.set α (Summarized (ListSegment δ))
+             (NodeTree.set δ (Point_to
+                  [(Int.zero,{|destination:=(γ,Int.zero);size:=AST.Mint32|});
+                     (add_chunk (Int.zero) AST.Mint32,{|destination:=(β,Int.zero);size:=AST.Mint32|})]
+                   )
+             (NodeTree.empty _)) ,
+             (Avar δ) ≠ 0)))
+      ])
+.
+
+Definition d : Summary.def :=
+  existT _ name def
+.
+
+Inductive fb := Forward | Backward.
+
+Definition list_unfoldings (i:name) : { U:Type & U -> unfolding name }:=
+  match i with
+  | List => existT _ (unit:Type) (fun _ => def List)
+  | ListSegment β => existT (fun U => U -> unfolding name) (fb:Type)
+                                 (fun d => match d with
+                                           | Forward => def (ListSegment β)
+                                           | Backward => list_segment_backward_unfolding β
+                                           end)
+  end
+.
+
+(* arnaud: WIP *)
+Program Definition env : Summary.env := {|
+  defs := d ;
+  unfoldings := list_unfoldings
+|}.
+Next Obligation. (** [defs_local] *)
+  unfold valuation_not_fixed_def, Valuation.central.
+  (** Reformulate the goal into a form where [lfp_ind] can be applied *)
+  cut (sub (Γ:=[names_of d;node;conc])
+             (γ d)
+             (fun i α s =>
+                forall β δ,
+                  ~ belongs_to_summary α i β ->
+                  ~ belongs_to_summary α i δ ->
+                  γ d i α (Valuation.swap β δ (fst s), (snd s)))).
+  { simpl; intros h; intros i α f β δ h₁ h₂ ν.
+    specialize (h i α (ν,f)); eauto. }
+  (** by induction *)
+  apply lfp_ind.
+  { typeclasses eauto. }
+  simpl; intros R h₁ h₂ i α [ν f] h₃ β δ hβ hδ; simpl.
+  change (lfp (F_γ d)) with (γ d) in h₁.
+  destruct i as [|γ].
+  - (** [List] *)
+    unfold F_γ,γ_unfolding in h₃.
+    rewrite <- γ_fixed_point.
+    unfold F_γ,γ_unfolding.
+    destruct h₃ as [ P [ εs [ r h₃]]]. exists P.
+    destruct h₃ as [ h₃₁ h₃₂ ].
+    destruct r as [ [ [[]|] | ] r_plus ].
+    * (** ν is of the form cons *)
+      simpl in * |-.
+      destruct r_plus as [ [] [ [] [] ]].
+      destruct (εs (Some None)) as [ [ε hε] ζ₀ ]; simpl in * |-; clear εs.
+      destruct (ζ₀ tt) as [ [ζ hζ] id_unit ]; simpl in * |-; clear ζ₀.
+      
+    * (** ν is of the form nil *)
+  - (** [ListSegment β] *)
